3 (10 marks) Show that B-splines of order 3 on {0,0,0,1,1,1} are second degree Berenstein polynomials.

The second degree berenstein polynomial:
$$ u^2 P_2 + (1-u)*u P_1 + (1-u)^2 P_0 $$

So for $i=0$:
\begin{align*}
N_{i=0,3}(u)
            &= \frac {u - 0} {0 - 0} \frac{u - 0} {0 - 0} % \tag{\text{ if ($ u_i \leq u \leq u_{i+1} $) } } \\
            &+ \frac {u - 0} {0 - 0} \frac{0 - u} {0 - 0} % \tag{\text{ if ( $u_{i+1} \leq u \leq u_{i+2}$ )}} \\
            &+ \frac {1 - u} { 1 - 0}\frac{u - 0} {0 - 0} % \tag{\text{ if ( $u_{i+2} \leq u \leq u_{i+3} $)}} \\
            &+ \frac {1 - u} { 1 - 0}\frac{0 - u} {0 - 0} % \tag{\text{ if ($ u_{i+3} \leq u \leq u_{i+4} $)}}
\end{align*}

%$ (  ( \frac { u - u_{0} }{ u_{ 2} - u_{0} })  (  ( \frac { u - u_{0} }{ u_{ 1} - u_{0} })  if ( u_i \leq  u \leq u_{i+1} ): 1   $ \\
%$ +  ( \frac { u_{2} - u }{ u_{ 2} - u_{1} })  if ( u_i \leq  u \leq u_{i+1} ): 1   ) $ \\
%$ +  ( \frac { u_{3} - u }{ u_{ 3} - u_{1} })  (  ( \frac { u - u_{1} }{ u_{ 2} - u_{1} })  if ( u_i \leq  u \leq u_{i+1} ): 1   $ \\
%$ +  ( \frac { u_{3} - u }{ u_{ 3} - u_{2} })  if ( u_i \leq  u \leq u_{i+1} ): 1   )  )$ \\

So for $i=1$:
\begin{align*}
N_{i=1,3}(u)
            &= \frac {u - u_{i}} {u_{i+2} - u_{i}} \frac{u - u_{i}} {u_{i+1} - u_{i}}  \tag{\text{ if ($ u_i \leq u \leq u_{i+1} $) } } \\
            &+ \frac {u - u_{i}} {u_{i+2} - u_{i}}  \frac{u_{i+2} - u } { u_{i+2} - u_{i+1}}  \tag{\text{ if ( $u_{i+1} \leq u \leq u_{i+2}$ )}} \\
            &+ \frac {u_{i+3} - u} { u_{i+3} - u_{i+1}} \frac {u - u_{i}} {u_{i+1} - u_{i}} \tag{\text{ if ( $u_{i+2} \leq u \leq u_{i+3} $)}} \\
            &+ \frac {u_{i+3} - u} { u_{i+3} - u_{i+1}} \frac{u_{i+2} - u } { u_{i+2} - u_{i+1} } \tag{\text{ if ($ u_{i+3} \leq u \leq u_{i+4} $)}}
            &= \frac {u - 0} {1 - 0} \frac{u - 0}  {0 - 0} \\
            &+ \frac {u - 0} {1 - 0} \frac{1 - u } { 1 - 0} \\
            &+ \frac {1 - u} {1 - 0} \frac{u - 0 } { 0 - 0} \\
%           &+ \frac {1 - u} {1 - 0} \frac{1 - u } { 1 - 0} \\
            &= u*(1-u) + (1-u)(1-u)
\end{align*}

%$ (  ( \frac { u - u_{0} }{ u_{ 2} - u_{0} })  (  ( \frac { u - u_{0} }{ u_{ 1} - u_{0} })  if ( u_i \leq  u \leq u_{i+1} ): 1    $\\
%$ +  ( \frac { u_{2} - u }{ u_{ 2} - u_{1} })  if ( u_i \leq  u \leq u_{i+1} ): 1   ) $ \\
%$ +  ( \frac { u_{3} - u }{ u_{ 3} - u_{1} })  (  ( \frac { u - u_{1} }{ u_{ 2} - u_{1} })  if ( u_i \leq  u \leq u_{i+1} ): 1   $ \\
%$ +  ( \frac { u_{3} - u }{ u_{ 3} - u_{2} })  if ( u_i \leq  u \leq u_{i+1} ): 1   )  )$

So for $i=2$:
\begin{align*}
N_{i=2,3}(u)
            &= \frac {u - u_{2}} {u_{4} - u_{2}} \frac{u - u_{2}} {u_{3} - u_{2}} \\
            &+ \frac {u - u_{2}} {u_{4} - u_{2}}  \frac{u_{4} - u } { u_{4} - u_{3}} \\
            &+ \frac {u_{5} - u} { u_{3} - u_{3}} \frac {u - u_{2}} {u_{3} - u_{2}} \\
            &+ \frac {u_{5} - u} { u_{3} - u_{3}} \frac{u_{4} - u } { u_{4} - u_{3} } \\
            &= \frac {u - 0} {1 - 0} \frac{u - 0} {1 - 0} \\
            &+ \frac {u - 0} {1 - 0} \frac{1 - u } { 1 - 1} \\
            &+ \frac {1 - u} { 1 - 1} \frac {u - 0} {1 - 0} \\
            &+ \frac {1 - u} { 1 - 1} \frac{1 - u } {1 - 1} 
            &= u*u + (1-u)*u + 0 + 0
\end{align*}

%$ (  ( \frac { u - u_{0} }{ u_{ 2} - u_{0} })  (  ( \frac { u - u_{0} }{ u_{ 1} - u_{0} })  if ( u_i \leq  u \leq u_{i+1} ): 1  $ \\
%$  +  ( \frac { u_{2} - u }{ u_{ 2} - u_{1} })  if ( u_i \leq  u \leq u_{i+1} ): 1   ) $ \\
%$  +  ( \frac { u_{3} - u }{ u_{ 3} - u_{1} })  (  ( \frac { u - u_{1} }{ u_{ 2} - u_{1} })  if ( u_i \leq  u \leq u_{i+1} ): 1   $ \\
%$ +  ( \frac { u_{3} - u }{ u_{ 3} - u_{2} })  if ( u_i \leq  u \leq u_{i+1} ): 1   )  ) $

Note: Due to the prior question mistakes, i=0, and i=1 is wrong.
